Mica/Stdlib/Combinators.lean
@@ -353,7 +353,7 @@ def matchType (inst : List (TinyML.TyVar × TinyML.Typ))
     match pattern, actual with
     | .tvar v, t => .ok (if inst.lookup v |>.isSome then inst else (v, t) :: inst)
     | .sum ps, .sum ts => matchTypes inst ps ts
-    | .arrow ps p, .arrow ts t => do
+    | .arrow ps p _, .arrow ts t _ => do
         let inst ← matchTypes inst ps ts
         matchType inst p t
     | .ref p, .ref t | .array p, .array t | .vec p, .vec t | .owned p, .owned t =>
